nrgqwörngjwr

Games/gameLib/Basic.lean
@@ -4,1049 +4,173 @@ Released under Apache 2.0 license as described in the file LICENSE.
 Author: Yves Jäckle.
 -/
 
-
-import Mathlib.Tactic
-import Games.exLib.Nat
-
--- should contain game structures, turn manipulations, history and state lemmas
+import Games.gameLib.TurnAPI
 
 
--- # Environments
+-- # Game worlds
 
-
-
-/--
-The game world for state type α and action type β.
--/
-structure Game_World (α β : Type u) where
-  /-- Inital state-/
+structure Game_World (α β : Type _) where
   init_game_state : α
-  /-- A predicate that decides in which states the game is won for the first player-/
-  fst_win_states : α → Prop
-  /-- A predicate that decides in which states the game is won for the second player-/
-  snd_win_states : α → Prop
-  /-- Given the initial state and the history, return a predicate
-  that determines the legal actions for the first player-/
-  fst_legal : α → List β → (β → Prop)
-  /-- Given the initial state and the history, return a predicate
-  that determines the legal actions for the second player-/
-  snd_legal : α → List β → (β → Prop)
-  /-- Given the initial state, the history, and an action of the frist player,
-  , and return next state-/
-  fst_transition : α → List β → β → α
-  /-- Given the initial state, the history, and an action of the second player,
-   and return next state-/
-  snd_transition : α → List β → β → α
+  fst_win_states : List β →  Prop
+  snd_win_states : List β → Prop
+  fst_legal : List β → (β → Prop)
+  snd_legal : List β → (β → Prop)
+  fst_transition : List β → β → α
+  snd_transition : List β → β → α
 
 
-/-- `Game_World` with addtional drawing states, given by a predicate on states-/
-structure Game_World_wDraw (α β : Type u) extends Game_World α β where
-  draw_states : α → Prop
+structure Game_World_wDraw (α β : Type _) extends Game_World α β where
+  draw_states : List β → Prop
 
 
-/--
-The game world for state type α and action type β, where players aren't discerened.
--/
-structure Symm_Game_World (α β : Type u) where
-  /-- Inital state-/
-  init_game_state : α
-  /-- A predicate that decides in which states the game is won for the players-/
-  win_states : α → Prop
-  /-- Given  the history, and an action of the player, return next state-/
-  transition : α → List β → β → α
-  /-- A predicate that decides in which states the game is won for the players-/
-  law : α → List β → (β → Prop)
-
-/-- `Symm_Game_World` with addtional drawing states, given by a predicate on states-/
-structure Symm_Game_World_wDraw (α β : Type u) extends Symm_Game_World α β where
-  draw_states : α → Prop
-
-/--
-Produce a `Game_World` from a `Symm_Game_World`.
--/
-def Symm_Game_World.toGame_World {α β : Type u} (g : Symm_Game_World α β) : Game_World α β :=
-  {init_game_state := g.init_game_state
-   fst_win_states := g.win_states
-   fst_transition := g.transition
-   fst_legal := g.law
-   snd_win_states := g.win_states
-   snd_transition := g.transition
-   snd_legal := g.law
-   }
-
-
-instance {α β : Type u} : Coe (Symm_Game_World α β) (Game_World α β) where
-  coe := Symm_Game_World.toGame_World
 
 @[simp]
-lemma Symm_Game_World.toGame_World_ini {α β : Type u} (g : Symm_Game_World α β) :
+lemma Game_World_wDraw.toGame_World_ini {α β : Type _} (g : Game_World_wDraw α β) :
   g.toGame_World.init_game_state = g.init_game_state :=
   by
   rfl
 
 @[simp]
-lemma Symm_Game_World.toGame_World_fst_win {α β : Type u} (g : Symm_Game_World α β) :
-  g.toGame_World.fst_win_states = g.win_states :=
+lemma Game_World_wDraw.toGame_World_fst_win {α β : Type _} (g : Game_World_wDraw α β) :
+  g.toGame_World.fst_win_states = g.fst_win_states :=
   by
   rfl
 
 @[simp]
-lemma Symm_Game_World.toGame_World_snd_win {α β : Type u} (g : Symm_Game_World α β) :
-  g.toGame_World.snd_win_states = g.win_states :=
+lemma Game_World_wDraw.toGame_World_snd_win {α β : Type _} (g : Game_World_wDraw α β) :
+  g.toGame_World.snd_win_states = g.snd_win_states :=
   by
   rfl
 
 @[simp]
-lemma Symm_Game_World.toGame_World_fst_trans {α β : Type u} (g : Symm_Game_World α β) :
+lemma Game_World_wDraw.toGame_World_fst_trans {α β : Type _} (g : Game_World_wDraw α β) :
+  g.toGame_World.fst_transition = g.fst_transition :=
+  by
+  rfl
+
+@[simp]
+lemma Game_World_wDraw.toGame_World_snd_trans {α β : Type _} (g : Game_World_wDraw α β) :
+  g.toGame_World.snd_transition = g.snd_transition :=
+  by
+  rfl
+
+@[simp]
+lemma Game_World_wDraw.toGame_World_fst_legal {α β : Type _} (g : Game_World_wDraw α β) :
+  g.toGame_World.fst_legal = g.fst_legal :=
+  by
+  rfl
+
+@[simp]
+lemma Game_World_wDraw.toGame_World_snd_legal {α β : Type _} (g : Game_World_wDraw α β) :
+  g.toGame_World.snd_legal = g.snd_legal :=
+  by
+  rfl
+
+
+structure Symm_Game_World (α β : Type _) where
+  init_game_state : α
+  fst_win_states : List β →  Prop
+  snd_win_states : List β → Prop
+  transition : List β → β → α
+  law : List β → (β → Prop)
+
+
+def Symm_Game_World.toGame_World {α β : Type _} (g : Symm_Game_World α β) : Game_World α β :=
+  {init_game_state := g.init_game_state
+   fst_win_states := g.fst_win_states
+   fst_transition := g.transition
+   fst_legal := g.law
+   snd_win_states := g.snd_win_states
+   snd_transition := g.transition
+   snd_legal := g.law
+   }
+
+
+instance {α β : Type _} : Coe (Symm_Game_World α β) (Game_World α β) where
+  coe := Symm_Game_World.toGame_World
+
+@[simp]
+lemma Symm_Game_World.toGame_World_ini {α β : Type _} (g : Symm_Game_World α β) :
+  g.toGame_World.init_game_state = g.init_game_state :=
+  by
+  rfl
+
+@[simp]
+lemma Symm_Game_World.toGame_World_fst_win {α β : Type _} (g : Symm_Game_World α β) :
+  g.toGame_World.fst_win_states = g.fst_win_states :=
+  by
+  rfl
+
+@[simp]
+lemma Symm_Game_World.toGame_World_snd_win {α β : Type _} (g : Symm_Game_World α β) :
+  g.toGame_World.snd_win_states = g.snd_win_states :=
+  by
+  rfl
+
+@[simp]
+lemma Symm_Game_World.toGame_World_fst_trans {α β : Type _} (g : Symm_Game_World α β) :
   g.toGame_World.fst_transition = g.transition :=
   by
   rfl
 
 @[simp]
-lemma Symm_Game_World.toGame_World_snd_trans {α β : Type u} (g : Symm_Game_World α β) :
+lemma Symm_Game_World.toGame_World_snd_trans {α β : Type _} (g : Symm_Game_World α β) :
   g.toGame_World.snd_transition = g.transition :=
   by
   rfl
 
 @[simp]
-lemma Symm_Game_World.toGame_World_fst_legal {α β : Type u} (g : Symm_Game_World α β) :
+lemma Symm_Game_World.toGame_World_fst_legal {α β : Type _} (g : Symm_Game_World α β) :
   g.toGame_World.fst_legal = g.law :=
   by
   rfl
 
 @[simp]
-lemma Symm_Game_World.toGame_World_snd_legal {α β : Type u} (g : Symm_Game_World α β) :
+lemma Symm_Game_World.toGame_World_snd_legal {α β : Type _} (g : Symm_Game_World α β) :
   g.toGame_World.snd_legal = g.law :=
   by
   rfl
 
 
+-- # Neutrality
 
-/--
-The list of actions represents the history of actions taken
-by both players. From the history and initial state (first input),
-one may deduce the current state, which may be used to define
-startegies. The output is the action to be played.
--/
-abbrev Strategy (α β : Type u) := α → List β → β
+structure Game_World.hist_neutral (g : Game_World α β) (hist : List β) : Prop where
+  not_fst : ¬ g.fst_win_states hist
+  not_snd : ¬ g.snd_win_states hist
 
+structure Game_World_wDraw.hist_neutral (g : Game_World_wDraw α β) (hist : List β) extends Game_World.hist_neutral g.toGame_World hist : Prop where
+  not_draw : ¬ g.draw_states hist
 
+def Symm_Game_World.hist_neutral (g : Symm_Game_World α β) (hist : List β) : Prop :=
+  g.toGame_World.hist_neutral hist
 
-/--
-Turn of the first player.
-Turn 0 represents initial state, then turns represent the state after the action-/
-def Turn_fst (turn : ℕ): Prop := turn % 2 = 1
 
-/--
-Turn of the decond player.
-Turn 0 represents initial state, then turns represent the state after the action-/
-def Turn_snd (turn : ℕ): Prop := ¬ (turn % 2 = 1)
 
-instance : DecidablePred Turn_fst :=
-  fun turn => by rw [Turn_fst] ; exact Nat.decEq (turn % 2) 1
 
-instance : DecidablePred Turn_snd :=
-  fun turn => by rw [Turn_snd] ; exact Not.decidable
+-- # Legality
 
-/-- The turn given the history-/
-abbrev Turn_from_hist {β : Type u} (hist : List β) := hist.length
-
-/-- The history of actions, given an initial state and the two startegies-/
-def History_on_turn {α β : Type u}
-    (ini : α) (fst_strat snd_strat: Strategy α β) : ℕ → List β
-| 0 => []
-| n+1 => let h := History_on_turn ini fst_strat snd_strat n
-         if Turn_fst (n+1)
-         then (fst_strat ini h) :: h
-         else (snd_strat ini h) :: h
-
-lemma History_on_turn_length {α β : Type u}
-    (ini : α) (fst_strat snd_strat: Strategy α β) (t : Nat) :
-    (History_on_turn ini fst_strat snd_strat t).length = t :=
-  by
-  induction' t with t ih
-  · dsimp [History_on_turn]
-  · dsimp [History_on_turn]
-    split_ifs <;> {rw [List.length_cons, ih]}
-
-
-/--
-FIX ME
-
-Given a law that returns a predicate on actions to determine legal actions,
-when provided an initial state and a history of actions on which the law may
-depend on, we define the notion of a strategy being legal (given another startegy).
-A strategy is legal if for all turns, the action for the history on that turn
-is legal wrt. the law at that history.
--/
-def Strategy_legal_fst {α β : Type u}
-  (ini : α) (f_law : α → List β → (β → Prop)) (f_strat s_strat : Strategy α β): Prop :=
-  ∀ turn : ℕ, Turn_fst (turn + 1) → f_law ini (History_on_turn ini f_strat s_strat turn) (f_strat ini (History_on_turn ini f_strat s_strat turn))
-      -- recall : turn is after the action
-
-/--
-FIX ME
--/
-def Strategy_legal_snd {α β : Type u}
-  (ini : α) (s_law : α → List β → (β → Prop)) (f_strat s_strat : Strategy α β): Prop :=
-  ∀ turn : ℕ, Turn_snd (turn +1) → s_law ini (History_on_turn ini f_strat s_strat turn) (s_strat ini (History_on_turn ini f_strat s_strat turn))
-      -- recall : turn is after the action
-
-
-/--
-A game is a game world extended by two specific strategies,
-and the certificates that they're legal wrt. the laws provided
-by the game world.
--/
-structure Game (α β : Type u) extends Game_World α β where
-  /-- The first players strategy-/
-  fst_strat : Strategy α β
-  /-- The second players strategy-/
-  snd_strat : Strategy α β
-  /-- The first players strategy is legal wrt. `fst_legal` and the second strategy-/
-  fst_lawful : Strategy_legal_fst init_game_state fst_legal fst_strat snd_strat
-  /-- The second players strategy is legal wrt. `snd_legal` and the first strategy-/
-  snd_lawful : Strategy_legal_snd init_game_state snd_legal fst_strat snd_strat
-
-/-- Same as `Game`, but for a symmetric game world-/
-structure Symm_Game (α β : Type u) extends Symm_Game_World α β where
-  /-- The first players strategy-/
-  fst_strat : Strategy α β
-  /-- The second players strategy-/
-  snd_strat : Strategy α β
-  /-- The first players strategy is legal wrt. `law` and the second strategy-/
-  fst_lawful : Strategy_legal_fst init_game_state law fst_strat snd_strat
-  /-- The second players strategy is legal wrt. `law` and the first strategy-/
-  snd_lawful : Strategy_legal_snd init_game_state law fst_strat snd_strat
-
-
-/-- Build a `Game` from a `Symm_Game`-/
-def Symm_Game.toGame {α β : Type u} (g : Symm_Game α β) : Game α β :=
- {init_game_state := g.init_game_state
-  fst_win_states := g.win_states
-  fst_transition := g.transition
-  fst_legal := g.law
-  snd_win_states := g.win_states
-  snd_transition := g.transition
-  snd_legal := g.law
-  fst_strat := g.fst_strat
-  fst_lawful := g.fst_lawful
-  snd_strat := g.snd_strat
-  snd_lawful := g.snd_lawful
-  }
-
-/-- ADD DOCS-/
-structure Game_wDraw (α β : Type u) extends Game_World_wDraw α β where
-  /-- The first players strategy-/
-  fst_strat : Strategy α β
-  /-- The second players strategy-/
-  snd_strat : Strategy α β
-  /-- The first players strategy is legal wrt. `fst_legal` and the second strategy-/
-  fst_lawful : Strategy_legal_fst init_game_state fst_legal fst_strat snd_strat
-  /-- The second players strategy is legal wrt. `snd_legal` and the first strategy-/
-  snd_lawful : Strategy_legal_snd init_game_state snd_legal fst_strat snd_strat
-
-
-
-@[simp]
-lemma Symm_Game.toGame_ini {α β : Type u} (g : Symm_Game α β) :
-  g.toGame.init_game_state = g.init_game_state :=
-  by
-  rfl
-
-@[simp]
-lemma Symm_Game.toGame_fst_win {α β : Type u} (g : Symm_Game α β) :
-  g.toGame.fst_win_states = g.win_states :=
-  by
-  rfl
-
-@[simp]
-lemma Symm_Game.toGame_snd_win {α β : Type u} (g : Symm_Game α β) :
-  g.toGame.snd_win_states = g.win_states :=
-  by
-  rfl
-
-@[simp]
-lemma Symm_Game.toGame_fst_trans {α β : Type u} (g : Symm_Game α β) :
-  g.toGame.fst_transition = g.transition :=
-  by
-  rfl
-
-@[simp]
-lemma Symm_Game.toGame_snd_trans {α β : Type u} (g : Symm_Game α β) :
-  g.toGame.snd_transition = g.transition :=
-  by
-  rfl
-
-@[simp]
-lemma Symm_Game.toGame_fst_legal {α β : Type u} (g : Symm_Game α β) :
-  g.toGame.fst_legal = g.law :=
-  by
-  rfl
-
-@[simp]
-lemma Symm_Game.toGame_snd_legal {α β : Type u} (g : Symm_Game α β) :
-  g.toGame.snd_legal = g.law :=
-  by
-  rfl
-
-@[simp]
-lemma Symm_Game.toGame_fst_strat {α β : Type u} (g : Symm_Game α β) :
-  g.toGame.fst_strat = g.fst_strat :=
-  by
-  rfl
-
-@[simp]
-lemma Symm_Game.toGame_snd_start {α β : Type u} (g : Symm_Game α β) :
-  g.toGame.snd_strat = g.snd_strat :=
-  by
-  rfl
-
-instance {α β : Type u} : Coe (Symm_Game α β) (Game α β) where
-  coe := Symm_Game.toGame
-
-
-@[simp]
-lemma Symm_Game.toSymm_Game_World_ini {α β : Type u} (g : Symm_Game α β) :
-  g.toSymm_Game_World.init_game_state = g.init_game_state :=
-  by
-  rfl
-
-
-
-@[simp]
-lemma Symm_Game.toGame_toWorld {α β : Type u} (g : Symm_Game α β):
-  g.toGame.toGame_World = g.toSymm_Game_World.toGame_World :=
-  by
-  dsimp [Symm_Game.toGame, Game.toGame_World, Symm_Game.toSymm_Game_World, Symm_Game_World.toGame_World]
-
-
-
-
-/-- History for a given turn, given a game world and stategies-/
-def Game_World.history_on_turn {α β : Type u} (g : Game_World α β)
-    (fst_strat snd_strat: Strategy α β) : ℕ → List β :=
-    History_on_turn g.init_game_state fst_strat snd_strat
-
-lemma Game_World.history_on_turn_def {α β : Type u} (g : Game_World α β) :
-    g.history_on_turn = History_on_turn g.init_game_state :=
-    by
-    rfl
-
-/-- History for a given turn, given a symmetric game world and stategies-/
-def Symm_Game_World.history_on_turn {α β : Type u} (g : Symm_Game_World α β)
-    (fst_strat snd_strat: Strategy α β) : ℕ → List β :=
-    History_on_turn g.init_game_state fst_strat snd_strat
-
-lemma Symm_Game_World.history_on_turn_def {α β : Type u} (g : Symm_Game_World α β):
-    g.history_on_turn = History_on_turn g.init_game_state :=
-    by
-    rfl
-
-
-/-- History for a given turn, given a game world and stategies-/
-def Game_World_wDraw.history_on_turn {α β : Type u} (g : Game_World_wDraw α β)
-    (fst_strat snd_strat: Strategy α β) : ℕ → List β :=
-    History_on_turn g.init_game_state fst_strat snd_strat
-
-lemma Game_World_wDraw.history_on_turn_def {α β : Type u} (g : Game_World_wDraw α β) :
-    g.history_on_turn = History_on_turn g.init_game_state :=
-    by
-    rfl
-
-@[simp]
-lemma History_on_turn_World_symm (g : Symm_Game_World α β):
-  g.toGame_World.history_on_turn = g.history_on_turn :=
-  by
-  funext f_st s_st
-  dsimp [Symm_Game_World.history_on_turn, Game_World.history_on_turn, Symm_Game_World.toGame_World]
-
-
-/-- Computes the history for a given turn, given a game-/
-def Game.history_on_turn {α β : Type u} (g : Game α β) : ℕ → List β :=
-  History_on_turn g.init_game_state g.fst_strat g.snd_strat
-
-lemma Game.history_on_turn_def {α β : Type u} (g : Game α β) :
-  g.history_on_turn = History_on_turn g.init_game_state g.fst_strat g.snd_strat :=
-  by
-  rfl
-
-/-- Computes the history for a given turn, given a symmetric game-/
-def Symm_Game.history_on_turn {α β : Type u} (g : Symm_Game α β) : ℕ → List β :=
-  History_on_turn g.init_game_state g.fst_strat g.snd_strat
-
-
-lemma Symm_Game.history_on_turn_def {α β : Type u} (g : Symm_Game α β) :
-  g.history_on_turn = History_on_turn g.init_game_state g.fst_strat g.snd_strat :=
-  by
-  rfl
-
-/-- Computes the history for a given turn, given a game-/
-def Game_wDraw.history_on_turn {α β : Type u} (g : Game_wDraw α β) : ℕ → List β :=
-  History_on_turn g.init_game_state g.fst_strat g.snd_strat
-
-lemma Game_wDraw.history_on_turn_def {α β : Type u} (g : Game_wDraw α β) :
-  g.history_on_turn = History_on_turn g.init_game_state g.fst_strat g.snd_strat :=
-  by
-  rfl
-
-@[simp]
-lemma History_on_turn_symm (g : Symm_Game α β):
-  g.toGame.history_on_turn = g.history_on_turn :=
-  by
-  dsimp [Symm_Game.history_on_turn, Game.history_on_turn, Symm_Game.toGame]
-
-@[simp]
-lemma History_on_turn_toWorld (g : Game α β):
-  g.toGame_World.history_on_turn g.fst_strat g.snd_strat = g.history_on_turn :=
-  by
-  dsimp [Game.history_on_turn, Game_World.history_on_turn, Game.toGame_World]
-
-@[simp]
-lemma History_on_turn_symm_toWorld (g : Symm_Game α β):
-  g.toSymm_Game_World.history_on_turn g.fst_strat g.snd_strat = g.history_on_turn :=
-  by
-  dsimp [Symm_Game.history_on_turn, Symm_Game_World.history_on_turn, Symm_Game.toSymm_Game_World]
-
-
-
-
--- # Turns
-
-
-
-lemma Turn_not_fst_iff_snd (turn : ℕ) : (¬ Turn_fst turn) ↔ Turn_snd turn :=
-  by rw [Turn_fst, Turn_snd]
-
-lemma Turn_not_snd_iff_fst (turn : ℕ) : (¬ Turn_snd turn) ↔ Turn_fst turn :=
-  by rw [Turn_fst, Turn_snd, not_ne_iff]
-
-lemma Turn_fst_or_snd (turn : ℕ) : Turn_fst turn ∨ Turn_snd turn :=
-  by rw [Turn_fst, Turn_snd] ; apply em
-
-
-lemma Turn_fst_step (turn : ℕ): Turn_fst turn ↔ Turn_fst (turn + 2) :=
-  by
-  constructor
-  · intro h
-    rw [Turn_fst] at *
-    rw [Nat.add_mod]
-    rw [h]
-    decide
-  · intro h
-    rw [Turn_fst] at *
-    rw [Nat.add_mod] at h
-    norm_num at h
-    exact h
-
-lemma Turn_snd_step (turn : ℕ): Turn_snd turn ↔ Turn_snd (turn + 2) :=
-  by
-  rw [← Turn_not_fst_iff_snd, ← Turn_not_fst_iff_snd]
-  rw [@not_iff_not]
-  apply Turn_fst_step
-
-lemma Turn_fst_snd_step (turn : ℕ): Turn_fst turn ↔ Turn_snd (turn + 1) :=
-  by
-  constructor
-  · intro h
-    rw [Turn_fst, Turn_snd] at *
-    rw [Nat.add_mod]
-    rw [h]
-    decide
-  · intro h
-    rw [Turn_fst, Turn_snd] at *
-    have := (or_iff_not_imp_right.mp (Nat.mod_two_eq_zero_or_one (turn+1))) h
-    rw [Nat.succ_mod_two_eq_zero_iff] at this
-    exact this
-
-
-lemma Turn_snd_fst_step (turn : ℕ): Turn_snd turn ↔ Turn_fst (turn + 1) :=
-  by
-  rw [← Turn_not_fst_iff_snd, ← @Turn_not_snd_iff_fst (turn + 1)]
-  rw [@not_iff_not]
-  apply Turn_fst_snd_step
-
-
-lemma Turn_fst_not_step (turn : ℕ): Turn_fst turn ↔ ¬ Turn_fst (turn + 1) :=
-  by
-  rw [Turn_not_fst_iff_snd]
-  apply Turn_fst_snd_step
-
-
-lemma Turn_snd_not_step (turn : ℕ): Turn_snd turn ↔ ¬ Turn_snd (turn + 1) :=
-  by
-  rw [Turn_not_snd_iff_fst]
-  apply Turn_snd_fst_step
-
-
-lemma Turn_add_fst_fst (a b : ℕ) : Turn_fst a → Turn_fst b → Turn_snd (a+b) :=
-  by
-  intro A B
-  dsimp [Turn_fst, Turn_snd] at *
-  rw [Nat.mod_two_ne_one, Nat.add_mod, A, B]
-  decide
-
-
-lemma Turn_add_fst_snd (a b : ℕ) : Turn_fst a → Turn_snd b → Turn_fst (a+b) :=
-  by
-  intro A B
-  dsimp [Turn_fst, Turn_snd] at *
-  rw [Nat.mod_two_ne_one] at B
-  rw [Nat.add_mod, A, B]
-  decide
-
-lemma Turn_add_snd_fst (a b : ℕ) : Turn_snd a → Turn_fst b → Turn_fst (a+b) :=
-  by
-  intro A B
-  dsimp [Turn_fst, Turn_snd] at *
-  rw [Nat.mod_two_ne_one] at A
-  rw [Nat.add_mod, A, B]
-  decide
-
-lemma Turn_add_snd_snd (a b : ℕ) : Turn_snd a → Turn_snd b → Turn_snd (a+b) :=
-  by
-  intro A B
-  dsimp [Turn_fst, Turn_snd] at *
-  rw [Nat.mod_two_ne_one] at *
-  rw [Nat.add_mod, A, B]
-  decide
-
-
-lemma History_on_turn_fst_to_snd (ini : α) (fst_strat snd_strat: Strategy α β) (turn : ℕ):
-  let H := History_on_turn ini fst_strat snd_strat ;
-  Turn_fst turn → H (turn + 1) = (snd_strat ini (H turn)) :: (H turn) :=
-  by
-  intro H tf
-  dsimp [H, History_on_turn]
-  rw [if_neg ((Turn_fst_not_step turn).mp tf)]
-
-lemma History_on_turn_snd_to_fst (ini : α) (fst_strat snd_strat: Strategy α β) (turn : ℕ):
-  let H := History_on_turn ini fst_strat snd_strat ;
-  Turn_snd turn → H (turn + 1) = (fst_strat ini (H turn)) :: (H turn) :=
-  by
-  intro H tf
-  dsimp [H, History_on_turn]
-  rw [if_pos ((Turn_snd_fst_step turn).mp tf)]
-
-lemma Symm_Game_World.history_on_turn_fst_to_snd
-  {α β : Type u} (g : Symm_Game_World α β)
-  (fst_strat snd_strat: Strategy α β) (turn : ℕ):
-  let H := g.history_on_turn fst_strat snd_strat ;
-  Turn_fst turn → H (turn + 1) = (snd_strat g.init_game_state (H turn)) :: (H turn) :=
-  by
-  intro H
-  dsimp [H, Symm_Game_World.history_on_turn]
-  apply History_on_turn_fst_to_snd
-
-lemma Symm_Game_World.history_on_turn_snd_to_fst
-  {α β : Type u} (g : Symm_Game_World α β)
-  (fst_strat snd_strat: Strategy α β) (turn : ℕ):
-  let H := g.history_on_turn fst_strat snd_strat ;
-  Turn_snd turn → H (turn + 1) = (fst_strat g.init_game_state (H turn)) :: (H turn) :=
-  by
-  intro H
-  dsimp [H, Symm_Game_World.history_on_turn]
-  apply History_on_turn_snd_to_fst
-
-
-lemma Game_World.history_on_turn_fst_to_snd
-  {α β : Type u} (g : Game_World α β)
-  (fst_strat snd_strat: Strategy α β) (turn : ℕ):
-  let H := g.history_on_turn fst_strat snd_strat ;
-  Turn_fst turn → H (turn + 1) = (snd_strat g.init_game_state (H turn)) :: (H turn) :=
-  by
-  intro H
-  dsimp [H, Game_World.history_on_turn]
-  apply History_on_turn_fst_to_snd
-
-lemma Game_World.history_on_turn_snd_to_fst
-  {α β : Type u} (g : Game_World α β)
-  (fst_strat snd_strat: Strategy α β) (turn : ℕ):
-  let H := g.history_on_turn fst_strat snd_strat ;
-  Turn_snd turn → H (turn + 1) = (fst_strat g.init_game_state (H turn)) :: (H turn) :=
-  by
-  intro H
-  dsimp [H, Game_World.history_on_turn]
-  apply History_on_turn_snd_to_fst
-
-
-lemma Game.history_on_turn_fst_to_snd
-  {α β : Type u} (g : Game α β) (turn : ℕ):
-  let H := g.history_on_turn ;
-  Turn_fst turn → H (turn + 1) = (g.snd_strat g.init_game_state (H turn)) :: (H turn) :=
-  by
-  intro H
-  dsimp [H, Game.history_on_turn]
-  apply History_on_turn_fst_to_snd
-
-lemma Game.history_on_turn_snd_to_fst
-  {α β : Type u} (g : Game α β) (turn : ℕ):
-  let H := g.history_on_turn ;
-  Turn_snd turn → H (turn + 1) = (g.fst_strat g.init_game_state (H turn)) :: (H turn) :=
-  by
-  intro H
-  dsimp [H, Game.history_on_turn]
-  apply History_on_turn_snd_to_fst
-
-lemma Symm_Game.history_on_turn_fst_to_snd
-  {α β : Type u} (g : Symm_Game α β) (turn : ℕ):
-  let H := g.history_on_turn ;
-  Turn_fst turn → H (turn + 1) = (g.snd_strat g.init_game_state (H turn)) :: (H turn) :=
-  by
-  intro H
-  dsimp [H, Symm_Game.history_on_turn]
-  apply History_on_turn_fst_to_snd
-
-lemma Symm_Game.history_on_turn_snd_to_fst
-  {α β : Type u} (g : Symm_Game α β) (turn : ℕ):
-  let H := g.history_on_turn ;
-  Turn_snd turn → H (turn + 1) = (g.fst_strat g.init_game_state (H turn)) :: (H turn) :=
-  by
-  intro H
-  dsimp [H, Symm_Game.history_on_turn]
-  apply History_on_turn_snd_to_fst
-
-
-/-- If a property is true on the first turn, and is maintained
-throughout the first players turns, then it is true for all the
-first players turns
--/
-lemma Invariant_fst {p : ℕ → Prop}
-  (bh : p 1) (ih : ∀ turn : ℕ, Turn_fst turn → p turn → p (turn + 2)):
-  ∀ turn : ℕ, Turn_fst turn → p turn :=
-  by
-  intro t
-  apply @Nat.induct_2_step _ t
-  · intro no
-    rw [Turn_fst] at no
-    contradiction
-  · intro
-    exact bh
-  · intro n a _ c
-    rw [← Turn_fst_step] at c
-    exact ih n c (a c)
-
-/-- If a property is true on the zeroth turn, and is maintained
-throughout the second players turns, then it is true for all the
-second players turns
--/
-lemma Invariant_snd {p : ℕ → Prop}
-  (bh : p 0) (ih : ∀ turn : ℕ, Turn_snd turn → p turn → p (turn + 2)):
-  ∀ turn : ℕ, Turn_snd turn → p turn :=
-  by
-  intro t
-  apply @Nat.induct_2_step _ t
-  swap
-  · intro no
-    rw [Turn_snd] at no
-    contradiction
-  · intro
-    exact bh
-  · intro n a _ c
-    rw [← Turn_snd_step] at c
-    exact ih n c (a c)
-
-
-/-- If a property is true on the second turn, and is maintained
-throughout the second players turns, then it is true for all the
-second players turns (except for maybe the zeroth).
--/
-lemma Invariant_snd' {p : ℕ → Prop}
-  (bh : p 2) (ih : ∀ turn : ℕ, Turn_snd turn → p turn → p (turn + 2)):
-  ∀ turn : ℕ, turn ≥ 2 → Turn_snd turn → p turn :=
-  by
-  intro t
-  apply @Nat.induct_2_step _ t
-  swap
-  · intro no nope
-    rw [Turn_snd] at nope
-    contradiction
-  · intro no
-    linarith
-  · intro n a _ b c
-    rw [← Turn_snd_step] at c
-    cases' n with m
-    · apply bh
-    · cases' m with k
-      · rw [Turn_snd] at c
-        contradiction
-      · apply ih
-        · apply c
-        · apply a _ c
-          rw [Nat.succ_eq_add_one]
-          linarith
-
-/--
-Given a game world and strategies, return the state given a turn
--/
-def Game_World.state_on_turn {α β : Type u} (g : Game_World α β)
-    (fst_strat snd_strat: Strategy α β) : ℕ → α
-| 0 => g.init_game_state
-| n+1 => let h := g.history_on_turn fst_strat snd_strat n
-         if Turn_fst (n+1)
-         then g.fst_transition g.init_game_state h (fst_strat g.init_game_state h)
-         else g.snd_transition g.init_game_state h (snd_strat g.init_game_state h)
-
-
-/--
-Given a game, return the state given a turn
--/
-def Game.state_on_turn {α β : Type u} (g : Game α β) : ℕ → α
-| 0 => g.init_game_state
-| n+1 => let h := g.history_on_turn n
-         if Turn_fst (n+1)
-         then g.fst_transition g.init_game_state h (g.fst_strat g.init_game_state h)
-         else g.snd_transition g.init_game_state h (g.snd_strat g.init_game_state h)
-
-
-lemma Game.state_on_turn_toWorld {α β : Type u} (g : Game α β):
-  g.toGame_World.state_on_turn g.fst_strat g.snd_strat = g.state_on_turn :=
-  by
-  funext n
-  dsimp [Game.state_on_turn, Game_World.state_on_turn]
-
-
-/--
-Given a symmetric game world and strategies, return the state given a turn
--/
-def Symm_Game_World.state_on_turn {α β : Type u} (g : Symm_Game_World α β)
-    (fst_strat snd_strat: Strategy α β) : ℕ → α
-| 0 => g.init_game_state
-| n+1 => let h := g.history_on_turn fst_strat snd_strat n
-         if Turn_fst (n+1)
-         then g.transition g.init_game_state h (fst_strat g.init_game_state h)
-         else g.transition g.init_game_state h (snd_strat g.init_game_state h)
-
-
-/--
-Given a symmetric game world and strategies, return the state given a turn
--/
-def Symm_Game.state_on_turn {α β : Type u} (g : Symm_Game α β) : ℕ → α
-| 0 => g.init_game_state
-| n+1 => let h := g.history_on_turn n
-         if Turn_fst (n+1)
-         then g.transition g.init_game_state h (g.fst_strat g.init_game_state h)
-         else g.transition g.init_game_state h (g.snd_strat g.init_game_state h)
-
-
-/--
-Given a game world and strategies, return the state given a turn
--/
-def Game_World_wDraw.state_on_turn {α β : Type u} (g : Game_World_wDraw α β)
-    (fst_strat snd_strat: Strategy α β) : ℕ → α
-| 0 => g.init_game_state
-| n+1 => let h := g.history_on_turn fst_strat snd_strat n
-         if Turn_fst (n+1)
-         then g.fst_transition g.init_game_state h (fst_strat g.init_game_state h)
-         else g.snd_transition g.init_game_state h (snd_strat g.init_game_state h)
-
-
-/--
-todo
--/
-lemma Game_World_wDraw.state_on_turn_toGame_World {α β : Type u} (g : Game_World_wDraw α β) :
-    g.state_on_turn = g.toGame_World.state_on_turn :=
-    by
-    rfl
-
-
-/--
-Given a game, return the state given a turn
--/
-def Game_wDraw.state_on_turn {α β : Type u} (g : Game_wDraw α β) : ℕ → α
-| 0 => g.init_game_state
-| n+1 => let h := g.history_on_turn n
-         if Turn_fst (n+1)
-         then g.fst_transition g.init_game_state h (g.fst_strat g.init_game_state h)
-         else g.snd_transition g.init_game_state h (g.snd_strat g.init_game_state h)
-
-
-lemma Symm_Game.state_on_turn_toWorld {α β : Type u} (g : Symm_Game α β):
-  g.toSymm_Game_World.state_on_turn g.fst_strat g.snd_strat = g.state_on_turn :=
-  by
-  funext n
-  dsimp [Symm_Game.state_on_turn, Symm_Game_World.state_on_turn]
-
-@[simp]
-lemma Symm_Game_World.state_on_turn_toGame_World {α β : Type u} (g : Symm_Game_World α β):
-  g.toGame_World.state_on_turn = g.state_on_turn :=
-  by
-  funext f s n
-  cases n with
-  | zero => dsimp [Game_World.state_on_turn, Symm_Game_World.state_on_turn]
-  | succ m =>
-      dsimp [Game_World.state_on_turn, Symm_Game_World.state_on_turn]
-      congr
-
-@[simp]
-lemma Symm_Game.state_on_turn_toGame {α β : Type u} (g : Symm_Game α β):
-  g.toGame.state_on_turn = g.state_on_turn :=
-  by
-  funext n
-  dsimp [Game.state_on_turn, Symm_Game.state_on_turn]
-
-
-
-lemma Game.state_on_turn_fst_to_snd
-  {α β : Type u} (g : Game α β) (turn : ℕ):
-  let S := g.state_on_turn ;
-  let H := g.history_on_turn turn ;
-  Turn_fst (turn + 1) → S (turn + 1) = g.fst_transition g.init_game_state H  (g.fst_strat g.init_game_state H) :=
-  by
-  intro S H t
-  dsimp [Game.state_on_turn]
-  rw [if_pos t]
-
-
-lemma Game.state_on_turn_snd_to_fst
-  {α β : Type u} (g : Game α β) (turn : ℕ):
-  let S := g.state_on_turn ;
-  let H := g.history_on_turn turn ;
-  Turn_snd (turn + 1) → S (turn + 1) = g.snd_transition g.init_game_state H  (g.snd_strat g.init_game_state H) :=
-  by
-  intro S H t
-  dsimp [Game.state_on_turn]
-  rw [← Turn_not_fst_iff_snd] at t
-  rw [if_neg t]
-
-lemma Symm_Game_World.state_on_turn_fst_to_snd
-  {α β : Type u} (g : Symm_Game_World α β) (f_strat s_strat : Strategy α β) (turn : ℕ):
-  let S := g.state_on_turn f_strat s_strat   ;
-  let H := History_on_turn g.init_game_state f_strat s_strat turn ;
-  Turn_fst (turn + 1) → S (turn + 1) = g.transition g.init_game_state H  (f_strat g.init_game_state H) :=
-  by
-  intro S H t
-  dsimp [Symm_Game_World.state_on_turn, Symm_Game_World.history_on_turn]
-  rw [if_pos t]
-
-lemma Symm_Game_World.state_on_turn_snd_to_fst
-  {α β : Type u} (g : Symm_Game_World α β) (f_strat s_strat : Strategy α β) (turn : ℕ):
-  let S := g.state_on_turn f_strat s_strat   ;
-  let H := History_on_turn g.init_game_state f_strat s_strat turn ;
-  Turn_snd (turn + 1) → S (turn + 1) = g.transition g.init_game_state H  (s_strat g.init_game_state H) :=
-  by
-  intro S H t
-  dsimp [Symm_Game_World.state_on_turn, Symm_Game_World.history_on_turn]
-  rw [if_neg (by exact t)]
-
-
-
-lemma Symm_Game.state_on_turn_fst_to_snd
-  {α β : Type u} (g : Symm_Game α β) (turn : ℕ):
-  let S := g.state_on_turn ;
-  let H := g.history_on_turn turn ;
-  Turn_fst (turn + 1) → S (turn + 1) = g.transition g.init_game_state H  (g.fst_strat g.init_game_state H) :=
-  by
-  intro S H t
-  dsimp [Symm_Game.state_on_turn]
-  rw [if_pos t]
-
-
-lemma Symm_Game.state_on_turn_snd_to_fst
-  {α β : Type u} (g : Symm_Game α β) (turn : ℕ):
-  let S := g.state_on_turn ;
-  let H := g.history_on_turn turn ;
-  Turn_snd (turn + 1) → S (turn + 1) = g.transition g.init_game_state H  (g.snd_strat g.init_game_state H) :=
-  by
-  intro S H t
-  dsimp [Symm_Game.state_on_turn]
-  rw [← Turn_not_fst_iff_snd] at t
-  rw [if_neg t]
-
-
-lemma Game_wDraw.state_on_turn_fst_to_snd
-  {α β : Type u} (g : Game_wDraw α β) (turn : ℕ):
-  let S := g.state_on_turn ;
-  let H := g.history_on_turn turn ;
-  Turn_fst (turn + 1) → S (turn + 1) = g.fst_transition g.init_game_state H  (g.fst_strat g.init_game_state H) :=
-  by
-  intro S H t
-  dsimp [Game_wDraw.state_on_turn]
-  rw [if_pos t]
-
-
-lemma Game_wDraw.state_on_turn_snd_to_fst
-  {α β : Type u} (g : Game_wDraw α β) (turn : ℕ):
-  let S := g.state_on_turn ;
-  let H := g.history_on_turn turn ;
-  Turn_snd (turn + 1) → S (turn + 1) = g.snd_transition g.init_game_state H  (g.snd_strat g.init_game_state H) :=
-  by
-  intro S H t
-  dsimp [Game_wDraw.state_on_turn]
-  rw [← Turn_not_fst_iff_snd] at t
-  rw [if_neg t]
-
-
-/-- The states from turn `0` to `turn - 1` -/
-def Game_World.state_upto_turn {α β : Type u} (g : Game_World α β)
-    (fst_strat snd_strat: Strategy α β) (turn : ℕ) : List α :=
-  List.map (g.state_on_turn fst_strat snd_strat) (List.range turn)
-
-/-- The states from turn `0` to `turn - 1` -/
-def Game.state_upto_turn {α β : Type u} (g : Game α β) (turn : ℕ) : List α :=
-  List.map g.state_on_turn (List.range turn)
-
-/-- The states from turn `0` to `turn - 1` -/
-def Symm_Game_World.state_upto_turn {α β : Type u} (g : Symm_Game_World α β)
-    (fst_strat snd_strat: Strategy α β) (turn : ℕ) : List α :=
-  List.map (g.state_on_turn fst_strat snd_strat) (List.range turn)
-
-/-- The states from turn `0` to `turn - 1` -/
-def Symm_Game.state_upto_turn {α β : Type u} (g : Symm_Game α β) (turn : ℕ) : List α :=
-  List.map g.state_on_turn (List.range turn)
-
-
-
-
--- # More
-
-lemma Symm_Game_World.mem_History_on_turn {α β : Type u}
-    (turn : ℕ)
-    (ini : α) (f_strat s_strat: Strategy α β)
-    (x : β) :
-    let H := History_on_turn ini f_strat s_strat ;
-    x ∈ H (turn) ↔ (∃ t < turn, ((Turn_fst (t+1) ∧ x = f_strat ini (H t)) ∨ (Turn_snd (t+1) ∧ x = s_strat ini (H t)))) :=
-    -- for ↑, recall that `f_strat ini (H t)` is the action of turn `t+1`
-    by
-    intro H
-    apply @Nat.strong_induction_on (fun turn => x ∈ H (turn) ↔ (∃ t < turn, (Turn_fst (t+1) ∧ x = f_strat ini (H t)) ∨ (Turn_snd (t+1) ∧ x = s_strat ini (H t)))) turn
-    intro n ih
-    cases' n with z s
-    · dsimp [H, History_on_turn]
-      simp only [List.not_mem_nil, not_lt_zero', false_and, exists_const]
-    · dsimp [H, History_on_turn]
-      split_ifs
-      · constructor
-        · intro c
-          rw [List.mem_cons] at c
-          cases' c with f hi
-          · use z
-            use (by exact Nat.le.refl)
-            left
-            rename_i l
-            exact ⟨l,f⟩
-          · specialize ih z (by exact Nat.le.refl)
-            obtain ⟨t, tl, tp⟩ := ih.mp hi
-            use t
-            use (by apply lt_trans tl ; exact Nat.lt.base z)
-        · rintro ⟨t,⟨tl,tp⟩⟩
-          rw [List.mem_cons]
-          cases' tp with f s
-          · specialize ih z (by exact Nat.le.refl)
-            by_cases q : t < z
-            · right
-              rw [ih]
-              use t
-              use q
-              left
-              exact f
-            · have : t = z := by exact Nat.eq_of_lt_succ_of_not_lt tl q
-              rw [this] at f
-              left
-              exact f.2
-          · specialize ih z (by exact Nat.le.refl)
-            by_cases q : t < z
-            · right
-              rw [ih]
-              use t
-              use q
-              right
-              exact s
-            · have : t = z := by exact Nat.eq_of_lt_succ_of_not_lt tl q
-              rw [this] at s
-              rename_i no
-              rw [← Turn_not_snd_iff_fst] at no
-              exfalso
-              exact no s.1
-      · constructor
-        · intro c
-          rw [List.mem_cons] at c
-          cases' c with f hi
-          · use z
-            use (by exact Nat.le.refl)
-            right
-            rename_i l
-            exact ⟨l,f⟩
-          · specialize ih z (by exact Nat.le.refl)
-            obtain ⟨t, tl, tp⟩ := ih.mp hi
-            use t
-            use (by apply lt_trans tl ; exact Nat.lt.base z)
-        · rintro ⟨t,⟨tl,tp⟩⟩
-          rw [List.mem_cons]
-          cases' tp with f s
-          · specialize ih z (by exact Nat.le.refl)
-            by_cases q : t < z
-            · right
-              rw [ih]
-              use t
-              use q
-              left
-              exact f
-            · have : t = z := by exact Nat.eq_of_lt_succ_of_not_lt tl q
-              rw [this] at f
-              rename_i no
-              exfalso
-              exact no f.1
-          · specialize ih z (by exact Nat.le.refl)
-            by_cases q : t < z
-            · right
-              rw [ih]
-              use t
-              use q
-              right
-              exact s
-            · have : t = z := by exact Nat.eq_of_lt_succ_of_not_lt tl q
-              rw [this] at s
-              left
-              exact s.2
-
-
-lemma History_on_turn_nonempty_of_succ
-  (ini : α) (f_strat s_strat: Strategy α β) {t : ℕ} :
-  History_on_turn ini f_strat s_strat (t+1) ≠ [] :=
-  by
-  dsimp [History_on_turn]
-  split_ifs <;> decide
-
-
-lemma History_on_turn_zero
-  (ini : α) (f_strat s_strat: Strategy α β) :
-  History_on_turn ini f_strat s_strat 0 = [] :=
-  by rfl
-
-lemma History_on_turn_getLast_fst_act (ini : α) (f_strat s_strat: Strategy α β) :
-  ∀ t : ℕ, (History_on_turn ini f_strat s_strat (t+1)).getLast (by apply History_on_turn_nonempty_of_succ)
-    = f_strat ini [] :=
-  by
-  intro t
-  induction' t with t ih
-  · dsimp [History_on_turn]
-    simp_rw [if_pos (show Turn_fst (0 + 1) from (by decide))]
-    dsimp [List.getLast]
-  · dsimp [History_on_turn] at *
-    by_cases  q : Turn_fst (Nat.succ t + 1)
-    · simp_rw [if_pos q]
-      rw [List.getLast_cons]
-      · exact ih
-    · simp_rw [if_neg q]
-      rw [List.getLast_cons]
-      · exact ih
-
-
-
-
-inductive Hist_legal (f_law s_law : α → List β → (β → Prop)) (ini : α) : List β → Prop
-| nil : Hist_legal f_law s_law ini []
+inductive Game_World.hist_legal (g : Game_World α β)  : List β → Prop
+| nil : g.hist_legal []
 | cons (l : List β) (act : β) : (if Turn_fst (l.length + 1)
-                                then f_law ini l act
-                                else s_law ini l act) → Hist_legal f_law s_law ini l →  Hist_legal f_law s_law ini (act :: l)
+                                then g.fst_legal l act
+                                else g.snd_legal l act) → g.hist_legal l →  g.hist_legal (act :: l)
 
-instance (f_law s_law : α → List β → (β → Prop)) [∀ i : α, ∀ h : List β, DecidablePred (f_law i h)] [∀ i : α, ∀ h : List β, DecidablePred (s_law i h)] (ini : α) : DecidablePred (Hist_legal f_law s_law ini) :=
+
+def Game_World_wDraw.hist_legal (g : Game_World_wDraw α β) (hist : List β) : Prop :=
+  g.toGame_World.hist_legal hist
+
+def Symm_Game_World.hist_legal (g : Symm_Game_World α β) (hist : List β) : Prop :=
+  g.toGame_World.hist_legal hist
+
+
+instance (g : Game_World α β)
+  [∀ h : List β, DecidablePred (g.fst_legal h)] [∀ h : List β, DecidablePred (g.snd_legal h)] :
+  DecidablePred (g.hist_legal) :=
   by
   intro hist
   induction' hist with x l ih
   · apply isTrue
-    apply Hist_legal.nil
+    apply Game_World.hist_legal.nil
   · cases' ih with ih ih
     · apply isFalse
       intro con
@@ -1056,7 +180,7 @@ instance (f_law s_law : α → List β → (β → Prop)) [∀ i : α, ∀ h : L
     · exact (if h : Turn_fst (l.length + 1)
              then (by
                    rename_i I I'
-                   specialize I ini l x
+                   specialize I l x
                    cases' I with I I
                    · apply isFalse
                      intro con
@@ -1065,13 +189,13 @@ instance (f_law s_law : α → List β → (β → Prop)) [∀ i : α, ∀ h : L
                      rw [if_pos h] at no
                      exact I no
                    · apply isTrue
-                     apply Hist_legal.cons _ _ _ ih
+                     apply Game_World.hist_legal.cons _ _ _ ih
                      rw [if_pos h]
                      exact I
                   )
              else (by
                    rename_i I I'
-                   specialize I' ini l x
+                   specialize I' l x
                    cases' I' with I' I'
                    · apply isFalse
                      intro con
@@ -1080,137 +204,82 @@ instance (f_law s_law : α → List β → (β → Prop)) [∀ i : α, ∀ h : L
                      rw [if_neg h] at no
                      exact I' no
                    · apply isTrue
-                     apply Hist_legal.cons _ _ _ ih
+                     apply Game_World.hist_legal.cons _ _ _ ih
                      rw [if_neg h]
                      exact I'))
 
 
-lemma Game_World.History_Hist_legal (g : Game_World α β)
-  (f_strat s_strat: Strategy α β)
-  (fst_lawful : Strategy_legal_fst g.init_game_state g.fst_legal f_strat s_strat)
-  (snd_lawful : Strategy_legal_snd g.init_game_state g.snd_legal f_strat s_strat)
-  (t : ℕ) :
-  Hist_legal g.fst_legal g.snd_legal g.init_game_state (History_on_turn g.init_game_state f_strat s_strat t) :=
-  by
-  induction' t with t ih
-  · dsimp [History_on_turn]
-    apply Hist_legal.nil
-  · dsimp [History_on_turn]
-    split_ifs
-    all_goals apply Hist_legal.cons _ _ _ ih
-    all_goals rename_i c
-    all_goals rw [History_on_turn_length]
-    · rw [if_pos c]
-      exact fst_lawful t c
-    · rw [if_neg c]
-      exact snd_lawful t c
 
-lemma Symm_Game_World.History_Hist_legal (g : Symm_Game_World α β)
-  (f_strat s_strat: Strategy α β)
-  (fst_lawful : Strategy_legal_fst g.init_game_state g.law f_strat s_strat)
-  (snd_lawful : Strategy_legal_snd g.init_game_state g.law f_strat s_strat)
-  (t : ℕ) :
-  Hist_legal g.law g.law g.init_game_state (History_on_turn g.init_game_state f_strat s_strat t) :=
-  by
-  induction' t with t ih
-  · dsimp [History_on_turn]
-    apply Hist_legal.nil
-  · dsimp [History_on_turn]
-    split_ifs
-    all_goals apply Hist_legal.cons _ _ _ ih
-    all_goals rename_i c
-    all_goals rw [History_on_turn_length]
-    · rw [if_pos c]
-      exact fst_lawful t c
-    · rw [if_neg c]
-      exact snd_lawful t c
+-- # Strategies
 
-lemma Game.History_Hist_legal (g : Game α β) (t : ℕ) :
-  Hist_legal g.fst_legal g.snd_legal g.init_game_state (History_on_turn g.init_game_state g.fst_strat g.snd_strat t) :=
-  by
-  apply Game_World.History_Hist_legal
-  · exact g.fst_lawful
-  · exact g.snd_lawful
+def Game_World.fStrategy (g : Game_World α β) :=
+  (hist : List β) → (Turn_fst (hist.length+1)) →
+  (g.hist_legal hist) → (g.hist_neutral hist) →
+  { act : β // g.fst_legal hist act}
+
+def Game_World.sStrategy (g : Game_World α β) :=
+  (hist : List β) → (Turn_snd (hist.length+1)) →
+  (g.hist_legal hist) → (g.hist_neutral hist) →
+  { act : β // g.snd_legal hist act}
+
+def Game_World_wDraw.fStrategy (g : Game_World_wDraw α β) :=
+  g.toGame_World.fStrategy
+
+def Game_World_wDraw.sStrategy (g : Game_World_wDraw α β) :=
+  g.toGame_World.sStrategy
+
+def Symm_Game_World.fStrategy (g : Symm_Game_World α β) :=
+  g.toGame_World.fStrategy
+
+def Symm_Game_World.sStrategy (g : Symm_Game_World α β) :=
+  g.toGame_World.sStrategy
 
 
 
-
--- # Carelessness
-
-def careless
-  (f_law s_law : α → List β → (β → Prop)) (ini : α)
-  (obj : α → List β → γ) (swap : α → List β → β → α): Prop :=
-  ∀ ini : α , ∀ hist : List β, ∀ prehist : List β, (h : prehist ≠ []) → Hist_legal f_law s_law ini prehist →
-    obj ini (hist ++ prehist) = obj (swap ini prehist.tail (prehist.head h)) hist
-
-lemma careless_singleton
-  (f_law s_law : α → List β → (β → Prop)) (ini : α)
-  (obj : α → List β → γ) (swap : α → List β → β → α) (hc : careless f_law s_law ini obj swap) :
-  ∀ ini : α , ∀ hist : List β, ∀ act : β, f_law ini [] act → obj ini (hist ++ [act]) = obj (swap ini [] (act)) hist
-  :=
-  by
-  intro ini hist act q
-  apply hc ini hist [act]
-  · apply List.noConfusion
-  · apply Hist_legal.cons
-    · rw [if_pos (by dsimp ; decide)]
-      exact q
-    · apply Hist_legal.nil
+-- # Histories
 
 
--- # More
-
-lemma History_eq_of_strat_strong_eq
-  (ini : α) (f_strat s_strat F_strat S_strat : Strategy α β)
-  (T : Nat)
-  (hf : ∀ hist : List β, hist.length ≤ T → f_strat ini hist = F_strat ini hist)
-  (hs : ∀ hist : List β, hist.length ≤ T → s_strat ini hist = S_strat ini hist) :
-  ∀ t ≤ (T+1), History_on_turn ini f_strat s_strat t = History_on_turn ini F_strat S_strat t :=
-  by
-  intro t tle
-  induction' t with t ih
-  · dsimp [History_on_turn]
-  · dsimp [History_on_turn]
-    by_cases q : Turn_fst (t + 1)
-    · rw [if_pos q, if_pos q]
-      specialize ih (by apply le_trans _ tle ; exact Nat.le.step Nat.le.refl)
-      rw [ih]
-      congr
-      apply hf
-      rw [History_on_turn_length]
-      exact Nat.lt_succ.mp tle
-    · rw [if_neg q, if_neg q]
-      specialize ih (by apply le_trans _ tle ; exact Nat.le.step Nat.le.refl)
-      rw [ih]
-      congr
-      apply hs
-      rw [History_on_turn_length]
-      exact Nat.lt_succ.mp tle
+inductive Game_World.hist_on_turn_output (g : Game_World α β) (t : Nat) where
+| invalid
+| terminal (result : {hist : List β // g.hist_legal hist ∧ hist.length = t})
+| nonterminal (result : {hist : List β // g.hist_legal hist ∧ hist.length = t}) (property : g.hist_neutral result.val)
 
 
-lemma History_eq_of_strat_strong_eq'
-  (ini : α) (f_strat s_strat F_strat S_strat : Strategy α β)
-  (T : Nat)
-  (hf : ∀ hist : List β, hist.length < T → f_strat ini hist = F_strat ini hist)
-  (hs : ∀ hist : List β, hist.length < T → s_strat ini hist = S_strat ini hist) :
-  ∀ t ≤ (T), History_on_turn ini f_strat s_strat t = History_on_turn ini F_strat S_strat t :=
-  by
-  intro t tle
-  induction' t with t ih
-  · dsimp [History_on_turn]
-  · dsimp [History_on_turn]
-    by_cases q : Turn_fst (t + 1)
-    · rw [if_pos q, if_pos q]
-      specialize ih (by apply le_trans _ tle ; exact Nat.le.step Nat.le.refl)
-      rw [ih]
-      congr
-      apply hf
-      rw [History_on_turn_length]
-      exact tle
-    · rw [if_neg q, if_neg q]
-      specialize ih (by apply le_trans _ tle ; exact Nat.le.step Nat.le.refl)
-      rw [ih]
-      congr
-      apply hs
-      rw [History_on_turn_length]
-      exact tle
+
+-- todo   instance Decidable (hist_neutral g [])
+
+
+open Classical in
+def Game_World.hist_on_turn (g : Game_World α β)
+  (fst_strat : g.fStrategy ) (snd_strat : g.sStrategy)
+  (t : ℕ) : g.hist_on_turn_output t :=
+  match t with
+  | 0 =>
+      if N : g.hist_neutral []
+      then
+        .nonterminal ⟨[], ⟨Game_World.hist_legal.nil, rfl⟩⟩ N
+      else
+        .terminal ⟨[], ⟨Game_World.hist_legal.nil, rfl⟩⟩
+  | n+1 =>  let h? := g.hist_on_turn fst_strat snd_strat n
+            match h? with
+            | .invalid | .terminal _ => .invalid
+            | .nonterminal h N =>
+            if T : Turn_fst (n+1)
+            then
+                let T' : Turn_fst (List.length h.val + 1) := by rw [h.property.2] ; exact T ;
+                let act := (fst_strat h.val T' h.property.1 N).val ;
+                let leg := (fst_strat h.val T' h.property.1 N).property ;
+                -- disjoin on whther win or not
+                ⟨ act :: h.val , ⟨Hist_legal.cons h.val act (by rw [if_pos T'] ; exact leg) h.property.1, (by dsimp ; rw [h.property.2])⟩⟩
+            else
+                let T' : Turn_snd (List.length h.val + 1) := by rw [Turn_snd_iff_not_fst , h.property.2] ; exact T ;
+                let act := (snd_strat h.val T' h.property.1).val ;
+                let leg := (snd_strat h.val T' h.property.1).property ;
+                ⟨ act :: h.val , ⟨Hist_legal.cons h.val act (by rw [if_neg ] ; exact leg ; rw [Turn_not_fst_iff_snd] ; exact T') h.property.1, (by dsimp ; rw [h.property.2])⟩⟩
+
+
+-- def Game_World.hist_on_turn_type (g : Game_World α β)
+--   (fst_strat : g.fStrategy ) (snd_strat : g.sStrategy) :
+--   Nat → Type _
+--   | 0 => {hist : List β // g.hist_legal hist ∧ hist.length = 0}
+--   | n+1 => (g.hist_neutral (Game_World.hist_on_turn g fst_strat snd_strat n).val) → {hist : List β // g.hist_legal hist ∧ hist.length = (n+1)}
