Games/gameLib/TurnAPI.lean
@@ -1,0 +1,156 @@
+/-
+Copyright (c) 2024 Yves Jäckle. All rights reserved.
+Released under Apache 2.0 license as described in the file LICENSE.
+Author: Yves Jäckle.
+-/
+
+
+import Mathlib.Tactic
+
+
+-- # Turns
+
+
+
+/--
+Turn of the first player.
+Turn 0 represents initial state, then turns represent the state after the action-/
+def Turn_fst (turn : ℕ): Prop := turn % 2 = 1
+
+/--
+Turn of the decond player.
+Turn 0 represents initial state, then turns represent the state after the action-/
+def Turn_snd (turn : ℕ): Prop := ¬ (turn % 2 = 1)
+
+
+instance : DecidablePred Turn_fst :=
+  fun turn => by rw [Turn_fst] ; exact Nat.decEq (turn % 2) 1
+
+instance : DecidablePred Turn_snd :=
+  fun turn => by rw [Turn_snd] ; exact Not.decidable
+
+
+
+lemma Turn_not_fst_iff_snd (turn : ℕ) : (¬ Turn_fst turn) ↔ Turn_snd turn :=
+  by rw [Turn_fst, Turn_snd]
+
+lemma Turn_not_snd_iff_fst (turn : ℕ) : (¬ Turn_snd turn) ↔ Turn_fst turn :=
+  by rw [Turn_fst, Turn_snd, not_ne_iff]
+
+lemma Turn_snd_iff_not_fst (turn : ℕ) : Turn_snd turn ↔ (¬ Turn_fst turn) :=
+  by rw [Turn_fst, Turn_snd]
+
+lemma Turn_fst_iff_not_snd (turn : ℕ) : Turn_fst turn ↔ (¬ Turn_snd turn) :=
+  by rw [Turn_fst, Turn_snd, not_ne_iff]
+
+lemma Turn_fst_or_snd (turn : ℕ) : Turn_fst turn ∨ Turn_snd turn :=
+  by rw [Turn_fst, Turn_snd] ; apply em
+
+
+lemma Turn_fst_step (turn : ℕ): Turn_fst turn ↔ Turn_fst (turn + 2) :=
+  by
+  simp_rw [Turn_fst] at *
+  rw [Nat.add_mod]
+  norm_num
+
+
+lemma Turn_snd_step (turn : ℕ): Turn_snd turn ↔ Turn_snd (turn + 2) :=
+  by
+  rw [← Turn_not_fst_iff_snd, ← Turn_not_fst_iff_snd, @not_iff_not]
+  apply Turn_fst_step
+
+lemma Turn_fst_snd_step (turn : ℕ): Turn_fst turn ↔ Turn_snd (turn + 1) :=
+  by
+  rw [Turn_fst, Turn_snd] at *
+  constructor
+  · intro h
+    rw [Nat.add_mod, h]
+    decide
+  · intro h
+    have := (or_iff_not_imp_right.mp (Nat.mod_two_eq_zero_or_one (turn+1))) h
+    rwa [Nat.succ_mod_two_eq_zero_iff] at this
+
+
+lemma Turn_snd_fst_step (turn : ℕ): Turn_snd turn ↔ Turn_fst (turn + 1) :=
+  by
+  rw [← Turn_not_fst_iff_snd, ← @Turn_not_snd_iff_fst (turn + 1), @not_iff_not]
+  apply Turn_fst_snd_step
+
+
+lemma Turn_fst_not_step (turn : ℕ): Turn_fst turn ↔ ¬ Turn_fst (turn + 1) :=
+  by
+  rw [Turn_not_fst_iff_snd]
+  apply Turn_fst_snd_step
+
+
+lemma Turn_snd_not_step (turn : ℕ): Turn_snd turn ↔ ¬ Turn_snd (turn + 1) :=
+  by
+  rw [Turn_not_snd_iff_fst]
+  apply Turn_snd_fst_step
+
+
+lemma Turn_not_fst_step (turn : ℕ): ¬ Turn_fst turn ↔ Turn_fst (turn + 1) :=
+  by
+  rw [not_iff_comm, Iff.comm , Turn_fst_not_step]
+
+
+
+lemma Turn_not_snd_step (turn : ℕ): ¬ Turn_snd turn ↔  Turn_snd (turn + 1) :=
+  by
+  rw [not_iff_comm, Iff.comm , Turn_snd_not_step]
+
+
+lemma Invariant_fst {p : ℕ → Prop}
+  (bh : p 1) (ih : ∀ turn : ℕ, Turn_fst turn → p turn → p (turn + 2)):
+  ∀ turn : ℕ, Turn_fst turn → p turn :=
+  by
+  intro t
+  apply Nat.twoStepInduction _ _ _ t
+  · intro no
+    rw [Turn_fst] at no
+    contradiction
+  · exact (fun _ => bh)
+  · intro n a _ c
+    rw [← Turn_fst_step] at c
+    exact ih n c (a c)
+
+
+lemma Invariant_snd {p : ℕ → Prop}
+  (bh : p 0) (ih : ∀ turn : ℕ, Turn_snd turn → p turn → p (turn + 2)):
+  ∀ turn : ℕ, Turn_snd turn → p turn :=
+  by
+  intro t
+  apply Nat.twoStepInduction _ _ _ t
+  swap
+  · intro no
+    rw [Turn_snd] at no
+    contradiction
+  · exact (fun _ => bh)
+  · intro n a _ c
+    rw [← Turn_snd_step] at c
+    exact ih n c (a c)
+
+lemma Invariant_snd' {p : ℕ → Prop}
+  (bh : p 2) (ih : ∀ turn : ℕ, Turn_snd turn → p turn → p (turn + 2)):
+  ∀ turn : ℕ, turn ≥ 2 → Turn_snd turn → p turn :=
+  by
+  intro t
+  apply Nat.twoStepInduction _ _ _ t
+  swap
+  · intro no nope
+    rw [Turn_snd] at nope
+    contradiction
+  · intro no
+    norm_num at no
+  · intro n a _ b c
+    rw [← Turn_snd_step] at c
+    cases' n with m
+    · apply bh
+    · cases' m with k
+      · rw [Turn_snd] at c
+        contradiction
+      · apply ih
+        · apply c
+        · apply a _ c
+          rw [Nat.succ_eq_add_one]
+          apply Nat.le_add_left
